engine/PrisonersDilemma.lean
@@ -1,5 +1,6 @@
 -- This module serves as the root of the `PrisonersDilemma` library.
 -- Import modules here that should be built as part of the library.
+import PrisonersDilemma.SizeLemmas
 import PrisonersDilemma.Theorems.CupodBot
 import PrisonersDilemma.Theorems.CooperateBot
 import PrisonersDilemma.Theorems.DefectBot
